YulSemanticsCommon.thy
@@ -1,0 +1,79 @@
+theory YulSemanticsCommon imports YulSyntax
+begin
+
+(* Primitives common to both small and big step Yul semantics *)
+datatype mode =
+  Regular
+  | Break
+  | Continue
+  | Leave
+
+datatype function_sig =
+  YulFunctionSig
+  (YulFunctionSigArguments: "YulTypedName list")
+  (YulFunctionSigReturnValues: "YulTypedName list")
+  (YulFunctionSigBody: "YulStatement list")
+
+type_synonym 'v locals = "YulIdentifier \<Rightarrow> 'v option"
+
+definition locals_empty :: "'v locals" where
+"locals_empty = (\<lambda> _ . None)"
+
+(* restrict e1 to the identifiers of e2 *)
+definition restrict :: "'v locals \<Rightarrow> 'v locals \<Rightarrow> 'v locals" where
+"restrict e1 e2 i =
+  (if e2 i = None then None
+      else e1 i)"
+
+fun strip_id_type :: "YulTypedName \<Rightarrow> YulIdentifier" where
+"strip_id_type (YulTypedName name type) = name"
+
+fun strip_id_types :: "YulTypedName list \<Rightarrow> YulIdentifier list" where
+"strip_id_types l =
+  List.map strip_id_type l"
+
+fun put_value :: "'v locals \<Rightarrow> YulIdentifier \<Rightarrow> 'v \<Rightarrow> 'v locals" where
+"put_value L i v =
+  (\<lambda> i' . if i' = i then Some v else L i')"
+
+fun put_values :: "'v locals \<Rightarrow> YulIdentifier list \<Rightarrow> 'v list \<Rightarrow> 'v locals option" where
+"put_values L [] [] = Some L"
+| "put_values L (ih#it) (vh#vt) =
+   (case put_values L it vt of
+    None \<Rightarrow> None
+    | Some L' \<Rightarrow> Some (put_value L' ih vh))"
+| "put_values L _ _ = None"
+
+fun get_values :: "'v locals \<Rightarrow> YulIdentifier list \<Rightarrow> 'v list option" where
+"get_values L ids =
+   List.those (List.map L (ids))"
+
+syntax plus_literal_inst.plus_literal :: "String.literal \<Rightarrow> String.literal \<Rightarrow> String.literal"
+  ("_ @@ _")
+
+record ('g, 'v) result =
+  global :: "'g"
+  locals :: "'v locals list"
+  funs :: "function_sig locals list"
+  mode :: "mode option"
+  vals :: "'v list option"
+
+datatype ('g, 'v) YulResult =
+  YulResult "('g, 'v) result"
+  | ErrorResult "String.literal"
+
+fun gatherYulFunctions :: "YulStatement list \<Rightarrow> ('g, 'v) YulResult \<Rightarrow> ('g, 'v) YulResult" where
+"gatherYulFunctions [] yr = yr"
+| "gatherYulFunctions 
+    ((YulFunctionDefinitionStatement (YulFunctionDefinition name args rets body))#t)
+     (YulResult r) =
+     (case funs r of
+      [] \<Rightarrow> ErrorResult (STR ''empty function context'')
+      | F#Ft \<Rightarrow>
+       gatherYulFunctions t
+        (YulResult (r \<lparr> funs := (put_value F name (YulFunctionSig args rets body) # Ft) \<rparr>)))"
+| "gatherYulFunctions (_#t) r =
+    gatherYulFunctions t r"
+
+
+end
